Defined events, knowledge functions and some lemmas for Smartphones

security-protocols/dap/EventSP.thy
@@ -8,72 +8,135 @@ consts  (*Initial states of agents -- parameter of the construction*)
 datatype smartphone = Smarphone agent
 
 datatype  
-  event = Says  agent agent msg
-        | Notes agent       msg
-        | Gets  agent       msg
-        | Shows agent       msg
-        | Scans smartphone agent msg 
+  event = Says    agent agent msg
+        | Notes   agent       msg
+        | Gets    agent       msg
+        | Inputs  agent       smartphone msg (* agent visually displays message to smartphone... *)
+        | Gets_s  smartphone  msg (* ... smartphone receives it *)
+        | Outputs smartphone  agent msg (* smartphone gives information to be inputed in agent... *)
+        | Gets_a  agent       msg (* ... agent receives it*)
     
 consts 
- bad     :: "agent set"  (* compromised agents *)
- stolen  :: "smartphone set" (* stolen smartphones *)
- secureM :: "bool" (* assumption of secure means between agents and their phones *)
+ bad        :: "agent set"  (* compromised agents *)
+ connected  :: "smartphone set" (* network connected smartphones *)
+ badp       :: "smartphone set" (* compromised smartphones *)
+ stolen     :: "smartphone set" (* stolen smartphones *)
 
 specification (bad)
   Spy_in_bad  [iff]: "Spy \<in> bad"
   Server_not_bad [iff]: "Server \<notin> bad"
   apply (rule exI [of _ "{Spy}"], simp)
   done
-
+  
 specification (stolen)
-  Phone_Server_not_stolen [iff]: "Smartphone Server \<notin> stolen"
-  Spy_Server_not_stolen [iff]: "Smartphone Spy \<notin> stolen"
+  Server_phone_not_stolen [iff]: "Smartphone Server \<notin> stolen"
+  Spy_phone_not_stolen [iff]: "Smartphone Spy \<notin> stolen"
   apply blast
   done
 
- 
+specification (badp)
+  (* Spy phone is secured because she already can use it freely *)
+  Spy_phone_in_bad [iff]: "Smartphone Spy \<notin> badp"  
+  Server_phone_not_bad [iff]: "Smartphone Server \<notin> badp"
+  apply blast
+  done
+
+(* Agents' knowledge definition over a trace is extended to comprehend new Smartphone events *)
+primrec knows :: "agent \<Rightarrow> event list \<Rightarrow> msg set" where
+  knows_Nil :  "knows A [] = initState A" |
+  knows_Cons : "knows A (ev # evs) =
+    (case ev of
+        Says A' B X \<Rightarrow> 
+          if (A = A' | A = Spy) then insert X (knows A evs)
+          else (knows A evs)
+      | Notes A' X \<Rightarrow>
+          if (A = A' | (A = Spy & A' \<in> bad)) then insert X (knows A evs)
+          else knows A evs
+      | Gets A' X \<Rightarrow>
+          if (A = A' & A \<noteq> Spy) then insert X (knows A evs)
+          else knows A evs
+      | Inputs A' P X \<Rightarrow>
+          if (A = A') then insert X (knows A evs)
+          else knows A evs
+      | Gets_s P X \<Rightarrow>
+          if (A = Spy & P \<in> connected & P \<in> badp) then insert X (knows A evs)
+          else knows A evs
+      | Outputs P A' X \<Rightarrow>
+          if (A = A' | (A = Spy & P \<in> connected & P \<in> badp)) then insert X (knows A evs)
+          else knows A evs
+      | Gets_a A' X \<Rightarrow>
+          if (A = A' & A \<noteq> Spy) then insert X (knows A evs)
+          else knows A evs
+  )"
+  
 primrec used :: "event list \<Rightarrow> msg set" where
-  used_Nil: "used [] = (\<Union> B. parts (initState B))" |
-  used_Cons: 
-    "used (ev # evs) = 
-      (case ev of   
-        Says A B X \<Rightarrow> parts {X} \<union> (used evs) |
-        Notes A X \<Rightarrow> parts {X} \<union> (used evs) |
-        Gets A X \<Rightarrow> used evs |
-        Shows P X \<Rightarrow> parts {X} \<union> (used evs) |
-        Scans P A X \<Rightarrow> parts {X} \<union> (used evs))" 
+  used_Nil  : "used [] = (\<Union> B. parts (initState B))" |
+  used_Cons : "used (ev # evs) = 
+    (case ev of   
+        Says A B X \<Rightarrow> parts {X} \<union> (used evs)
+      | Notes A X \<Rightarrow> parts {X} \<union> (used evs)
+      | Gets A X \<Rightarrow> used evs
+      | Inputs A P X \<Rightarrow> parts {X} \<union> used evs
+      | Gets_s P X \<Rightarrow> used evs
+      | Outputs P A X \<Rightarrow> parts {X} \<union> used evs
+      | Gets_a A X \<Rightarrow> used evs
+  )" 
 
-lemma Notes_imp_used [rule_format]: "Notes A X \<in> set evs --> X \<in> used evs"
+
+  
+lemma Notes_imp_used [rule_format] : 
+  "Notes A X \<in> set evs \<longrightarrow> X \<in> used evs"
 apply (induct_tac evs)
 apply (auto split: event.split) 
 done
 
-lemma Says_imp_used [rule_format]: "Says A B X \<in> set evs --> X \<in> used evs"
-apply (induct_tac evs)
-apply (auto split: event.split) 
-done
-
-lemma MPair_used [rule_format]:
-     "MPair X Y \<in> used evs --> X \<in> used evs & Y \<in> used evs"
+lemma Says_imp_used [rule_format] :
+  "Says A B X \<in> set evs \<longrightarrow> X \<in> used evs"
 apply (induct_tac evs)
 apply (auto split: event.split) 
 done
 
 
 
-(* primrec knows :: "agent \<Rightarrow> event list \<Rightarrow> msg set" where
-  knows_Nil: "knows A [] = initState A" |
-  knows_Cons: 
-    "knows A (ev # evs) = (case ev of
-      Says A' B X \<Rightarrow>
-        if (A = A' | A = Spy) then insert X (knows A evs) else knows A evs |
-      Notes A' X \<Rightarrow>
-        if (A = A' | (A = Spy & A' \<in> bad)) then insert X (knows A evs) else knows A evs |
-      Gets A' X \<Rightarrow>
-        if (A = A' & A \<noteq> Spy) then insert X (knows A evs) else knows A evs |
-      Shows A' X \<Rightarrow>
-        if (A = A' | A = Spy) then insert X (knows A evs) else knows A evs |
-      Scans P A' X \<Rightarrow> 
-        if () )"
-*)             
+
+lemmas parts_insert_knows_A = parts_insert [of _ "knows A evs"] for A evs
+
+lemma knows_Spy_Says [simp] :
+  "knows Spy (Says A B X # evs) = insert X (knows Spy evs)"
+by simp
+
+lemma knows_Spy_Gets [simp] :
+  "knows Spy (Gets B X # evs) = knows Spy evs"
+by simp
+
+lemma knows_Spy_Notes [simp] : 
+  "knows Spy (Notes A X # evs) = 
+    (if A \<in> bad then insert X (knows Spy evs) else knows Spy evs)"
+by simp
+
+lemma knows_Spy_Inputs [simp] : 
+  "knows Spy (Inputs A P X # evs) = 
+    (if A = Spy then insert X (knows Spy evs) else knows Spy evs)"
+by simp
+
+lemma knows_Spy_Gets_s [simp] :
+  "knows Spy (Gets_s P X # evs) = 
+    (if (P \<in> connected & P \<in> badp) then insert X (knows Spy evs) else knows Spy evs)"
+by simp
+
+lemma knows_Spy_Outputs [simp] : 
+  "knows Spy (Outputs P A X # evs) = 
+    (
+      if A = Spy then insert X (knows Spy evs)
+      else if (P \<in> connected & P \<in> badp) then insert X (knows Spy evs)
+      else knows Spy evs
+    )"
+by simp
+
+lemma knows_Spy_Gets_a [simp] :
+  "knows Spy (Gets_a A X # evs) = knows Spy evs"
+by simp
+
+
+
 end
